WebAssembly/Wasm_Soundness.thy
@@ -7,12 +7,15 @@ theorem preservation:
           "\<lparr>s;vs;es\<rparr> \<leadsto>_i \<lparr>s';vs';es'\<rparr>"
   shows "\<turnstile>_i s';vs';es' : ts"
 proof -
-  obtain \<S> where "store_typing s \<S>" "\<S>\<bullet>None \<tturnstile>_i vs;es : ts"
+  have "store_typing s" "s\<bullet>None \<tturnstile>_i vs;es : ts"
     using assms(1) config_typing.simps
-    by blast
-  hence "store_typing s' \<S>" "\<S>\<bullet>None \<tturnstile>_i vs';es' : ts"
-    using assms(2) store_preserved types_preserved_e
-    by simp_all
+    by blast+
+  hence "store_typing s'" "s'\<bullet>None \<tturnstile>_i vs';es' : ts"
+    using assms(2)
+          store_preserved
+          types_preserved_e
+          store_extension_imp_store_typing
+    by blast+
   thus ?thesis
     using config_typing.intros
     by blast
@@ -22,9 +25,9 @@ theorem progress:
   assumes "\<turnstile>_i s;vs;es : ts"
   shows "const_list es \<or> es = [Trap] \<or> (\<exists>a s' vs' es'. \<lparr>s;vs;es\<rparr> \<leadsto>_i \<lparr>s';vs';es'\<rparr>)"
 proof -
-  obtain \<S> where "store_typing s \<S>" "\<S>\<bullet>None \<tturnstile>_i vs;es : ts"
+  have "store_typing s" "s\<bullet>None \<tturnstile>_i vs;es : ts"
     using assms config_typing.simps
-    by blast
+    by blast+
   thus ?thesis
     using progress_e3
     by blast
